src/Corecursive_Prop.thy
@@ -194,8 +194,8 @@ text \<open>
 \<close>
 lemma TESL_interp_stepwise_sporadicon_coind_unfold:
   \<open>\<lbrakk> K\<^sub>1 sporadic \<tau> on K\<^sub>2 \<rbrakk>\<^sub>T\<^sub>E\<^sub>S\<^sub>L\<^bsup>\<ge> n\<^esup> =
-    \<lbrakk> K\<^sub>1 \<Up> n \<rbrakk>\<^sub>p\<^sub>r\<^sub>i\<^sub>m \<inter> \<lbrakk> K\<^sub>2 \<Down> n @ \<tau> \<rbrakk>\<^sub>p\<^sub>r\<^sub>i\<^sub>m        \<comment> \<open>rule @{thm sporadic_on_e2}\<close>
-    \<union> \<lbrakk> K\<^sub>1 sporadic \<tau> on K\<^sub>2 \<rbrakk>\<^sub>T\<^sub>E\<^sub>S\<^sub>L\<^bsup>\<ge> Suc n\<^esup>\<close>   \<comment> \<open>rule @{thm sporadic_on_e1}\<close>
+    \<lbrakk> K\<^sub>1 \<Up> n \<rbrakk>\<^sub>p\<^sub>r\<^sub>i\<^sub>m \<inter> \<lbrakk> K\<^sub>2 \<Down> n @ \<tau> \<rbrakk>\<^sub>p\<^sub>r\<^sub>i\<^sub>m        \<comment> \<open>rule @{term sporadic_on_e2}\<close>
+    \<union> \<lbrakk> K\<^sub>1 sporadic \<tau> on K\<^sub>2 \<rbrakk>\<^sub>T\<^sub>E\<^sub>S\<^sub>L\<^bsup>\<ge> Suc n\<^esup>\<close>   \<comment> \<open>rule @{term sporadic_on_e1}\<close>
 unfolding TESL_interpretation_atomic_stepwise.simps(1)
           symbolic_run_interpretation_primitive.simps(1,6)
 using exists_nat_set_suc[of \<open>n\<close> \<open>\<lambda>\<rho> n. hamlet (Rep_run \<rho> n K\<^sub>1)
@@ -204,7 +204,7 @@ by (simp add: Collect_conj_eq)
 
 
 lemma TESL_interp_stepwise_tagrel_coind_unfold:
-  \<open>\<lbrakk> time-relation \<lfloor>K\<^sub>1, K\<^sub>2\<rfloor> \<in> R \<rbrakk>\<^sub>T\<^sub>E\<^sub>S\<^sub>L\<^bsup>\<ge> n\<^esup> =        \<comment> \<open>rule @{thm tagrel_e}\<close>
+  \<open>\<lbrakk> time-relation \<lfloor>K\<^sub>1, K\<^sub>2\<rfloor> \<in> R \<rbrakk>\<^sub>T\<^sub>E\<^sub>S\<^sub>L\<^bsup>\<ge> n\<^esup> =        \<comment> \<open>rule @{term tagrel_e}\<close>
      \<lbrakk> \<lfloor>\<tau>\<^sub>v\<^sub>a\<^sub>r(K\<^sub>1, n), \<tau>\<^sub>v\<^sub>a\<^sub>r(K\<^sub>2, n)\<rfloor> \<in> R \<rbrakk>\<^sub>p\<^sub>r\<^sub>i\<^sub>m
      \<inter> \<lbrakk> time-relation \<lfloor>K\<^sub>1, K\<^sub>2\<rfloor> \<in> R \<rbrakk>\<^sub>T\<^sub>E\<^sub>S\<^sub>L\<^bsup>\<ge> Suc n\<^esup>\<close>
 proof -
@@ -218,8 +218,8 @@ qed
 
 lemma TESL_interp_stepwise_implies_coind_unfold:
   \<open>\<lbrakk> master implies slave \<rbrakk>\<^sub>T\<^sub>E\<^sub>S\<^sub>L\<^bsup>\<ge> n\<^esup> =
-     (   \<lbrakk> master \<not>\<Up> n \<rbrakk>\<^sub>p\<^sub>r\<^sub>i\<^sub>m                     \<comment> \<open>rule @{thm implies_e1}\<close>
-       \<union> \<lbrakk> master \<Up> n \<rbrakk>\<^sub>p\<^sub>r\<^sub>i\<^sub>m \<inter> \<lbrakk> slave \<Up> n \<rbrakk>\<^sub>p\<^sub>r\<^sub>i\<^sub>m)  \<comment> \<open>rule @{thm implies_e2}\<close>
+     (   \<lbrakk> master \<not>\<Up> n \<rbrakk>\<^sub>p\<^sub>r\<^sub>i\<^sub>m                     \<comment> \<open>rule @{term implies_e1}\<close>
+       \<union> \<lbrakk> master \<Up> n \<rbrakk>\<^sub>p\<^sub>r\<^sub>i\<^sub>m \<inter> \<lbrakk> slave \<Up> n \<rbrakk>\<^sub>p\<^sub>r\<^sub>i\<^sub>m)  \<comment> \<open>rule @{term implies_e2}\<close>
      \<inter> \<lbrakk> master implies slave \<rbrakk>\<^sub>T\<^sub>E\<^sub>S\<^sub>L\<^bsup>\<ge> Suc n\<^esup>\<close>
 proof -
   have \<open>{\<rho>. \<forall>m\<ge>n. hamlet ((Rep_run \<rho>) m master) \<longrightarrow> hamlet ((Rep_run \<rho>) m slave)}
@@ -233,8 +233,8 @@ qed
 
 lemma TESL_interp_stepwise_implies_not_coind_unfold:
   \<open>\<lbrakk> master implies not slave \<rbrakk>\<^sub>T\<^sub>E\<^sub>S\<^sub>L\<^bsup>\<ge> n\<^esup> =
-     (    \<lbrakk> master \<not>\<Up> n \<rbrakk>\<^sub>p\<^sub>r\<^sub>i\<^sub>m                       \<comment> \<open>rule @{thm implies_not_e1}\<close>
-        \<union> \<lbrakk> master \<Up> n \<rbrakk>\<^sub>p\<^sub>r\<^sub>i\<^sub>m \<inter> \<lbrakk> slave \<not>\<Up> n \<rbrakk>\<^sub>p\<^sub>r\<^sub>i\<^sub>m)  \<comment> \<open>rule @{thm implies_not_e2}\<close>
+     (    \<lbrakk> master \<not>\<Up> n \<rbrakk>\<^sub>p\<^sub>r\<^sub>i\<^sub>m                       \<comment> \<open>rule @{term implies_not_e1}\<close>
+        \<union> \<lbrakk> master \<Up> n \<rbrakk>\<^sub>p\<^sub>r\<^sub>i\<^sub>m \<inter> \<lbrakk> slave \<not>\<Up> n \<rbrakk>\<^sub>p\<^sub>r\<^sub>i\<^sub>m)  \<comment> \<open>rule @{term implies_not_e2}\<close>
      \<inter> \<lbrakk> master implies not slave \<rbrakk>\<^sub>T\<^sub>E\<^sub>S\<^sub>L\<^bsup>\<ge> Suc n\<^esup>\<close>
 proof -
   have \<open>{\<rho>. \<forall>m\<ge>n. hamlet ((Rep_run \<rho>) m master) \<longrightarrow> \<not> hamlet ((Rep_run \<rho>) m slave)}
@@ -248,9 +248,9 @@ qed
 
 lemma TESL_interp_stepwise_timedelayed_coind_unfold:
   \<open>\<lbrakk> master time-delayed by \<delta>\<tau> on measuring implies slave \<rbrakk>\<^sub>T\<^sub>E\<^sub>S\<^sub>L\<^bsup>\<ge> n\<^esup> =
-     (     \<lbrakk> master \<not>\<Up> n \<rbrakk>\<^sub>p\<^sub>r\<^sub>i\<^sub>m               \<comment> \<open>rule @{thm timedelayed_e1}\<close>
+     (     \<lbrakk> master \<not>\<Up> n \<rbrakk>\<^sub>p\<^sub>r\<^sub>i\<^sub>m               \<comment> \<open>rule @{term timedelayed_e1}\<close>
         \<union> (\<lbrakk> master \<Up> n \<rbrakk>\<^sub>p\<^sub>r\<^sub>i\<^sub>m \<inter> \<lbrakk> measuring @ n \<oplus> \<delta>\<tau> \<Rightarrow> slave \<rbrakk>\<^sub>p\<^sub>r\<^sub>i\<^sub>m))
-                                             \<comment> \<open>rule @{thm timedelayed_e2}\<close>
+                                             \<comment> \<open>rule @{term timedelayed_e2}\<close>
      \<inter> \<lbrakk> master time-delayed by \<delta>\<tau> on measuring implies slave \<rbrakk>\<^sub>T\<^sub>E\<^sub>S\<^sub>L\<^bsup>\<ge> Suc n\<^esup>\<close>
 proof -
   let ?prop = \<open>\<lambda>\<rho> m. hamlet ((Rep_run \<rho>) m master) \<longrightarrow>
@@ -266,7 +266,7 @@ proof -
 qed
 
 lemma TESL_interp_stepwise_weakly_precedes_coind_unfold:
-   \<open>\<lbrakk> K\<^sub>1 weakly precedes K\<^sub>2 \<rbrakk>\<^sub>T\<^sub>E\<^sub>S\<^sub>L\<^bsup>\<ge> n\<^esup> =                 \<comment> \<open>rule @{thm weakly_precedes_e}\<close>
+   \<open>\<lbrakk> K\<^sub>1 weakly precedes K\<^sub>2 \<rbrakk>\<^sub>T\<^sub>E\<^sub>S\<^sub>L\<^bsup>\<ge> n\<^esup> =                 \<comment> \<open>rule @{term weakly_precedes_e}\<close>
       \<lbrakk> (\<lceil>#\<^sup>\<le> K\<^sub>2 n, #\<^sup>\<le> K\<^sub>1 n\<rceil> \<in> (\<lambda>(x,y). x\<le>y)) \<rbrakk>\<^sub>p\<^sub>r\<^sub>i\<^sub>m 
       \<inter> \<lbrakk> K\<^sub>1 weakly precedes K\<^sub>2 \<rbrakk>\<^sub>T\<^sub>E\<^sub>S\<^sub>L\<^bsup>\<ge> Suc n\<^esup>\<close>
 proof -
@@ -280,7 +280,7 @@ proof -
 qed
 
 lemma TESL_interp_stepwise_strictly_precedes_coind_unfold:
-   \<open>\<lbrakk> K\<^sub>1 strictly precedes K\<^sub>2 \<rbrakk>\<^sub>T\<^sub>E\<^sub>S\<^sub>L\<^bsup>\<ge> n\<^esup> =               \<comment> \<open>rule @{thm strictly_precedes_e}\<close>
+   \<open>\<lbrakk> K\<^sub>1 strictly precedes K\<^sub>2 \<rbrakk>\<^sub>T\<^sub>E\<^sub>S\<^sub>L\<^bsup>\<ge> n\<^esup> =               \<comment> \<open>rule @{term strictly_precedes_e}\<close>
       \<lbrakk> (\<lceil>#\<^sup>\<le> K\<^sub>2 n, #\<^sup>< K\<^sub>1 n\<rceil> \<in> (\<lambda>(x,y). x\<le>y)) \<rbrakk>\<^sub>p\<^sub>r\<^sub>i\<^sub>m
       \<inter> \<lbrakk> K\<^sub>1 strictly precedes K\<^sub>2 \<rbrakk>\<^sub>T\<^sub>E\<^sub>S\<^sub>L\<^bsup>\<ge> Suc n\<^esup>\<close>
 proof -
@@ -295,8 +295,8 @@ qed
 
 lemma TESL_interp_stepwise_kills_coind_unfold:
    \<open>\<lbrakk> K\<^sub>1 kills K\<^sub>2 \<rbrakk>\<^sub>T\<^sub>E\<^sub>S\<^sub>L\<^bsup>\<ge> n\<^esup> =
-      (   \<lbrakk> K\<^sub>1 \<not>\<Up> n \<rbrakk>\<^sub>p\<^sub>r\<^sub>i\<^sub>m                        \<comment> \<open>rule @{thm kills_e1}\<close>
-        \<union> \<lbrakk> K\<^sub>1 \<Up> n \<rbrakk>\<^sub>p\<^sub>r\<^sub>i\<^sub>m \<inter> \<lbrakk> K\<^sub>2 \<not>\<Up> \<ge> n \<rbrakk>\<^sub>p\<^sub>r\<^sub>i\<^sub>m)    \<comment> \<open>rule @{thm kills_e2}\<close>
+      (   \<lbrakk> K\<^sub>1 \<not>\<Up> n \<rbrakk>\<^sub>p\<^sub>r\<^sub>i\<^sub>m                        \<comment> \<open>rule @{term kills_e1}\<close>
+        \<union> \<lbrakk> K\<^sub>1 \<Up> n \<rbrakk>\<^sub>p\<^sub>r\<^sub>i\<^sub>m \<inter> \<lbrakk> K\<^sub>2 \<not>\<Up> \<ge> n \<rbrakk>\<^sub>p\<^sub>r\<^sub>i\<^sub>m)    \<comment> \<open>rule @{term kills_e2}\<close>
       \<inter> \<lbrakk> K\<^sub>1 kills K\<^sub>2 \<rbrakk>\<^sub>T\<^sub>E\<^sub>S\<^sub>L\<^bsup>\<ge> Suc n\<^esup>\<close>
 proof -
   let ?kills = \<open>\<lambda>n \<rho>. \<forall>p\<ge>n. hamlet ((Rep_run \<rho>) p K\<^sub>1)
@@ -398,7 +398,7 @@ by (simp add: TESL_interp_stepwise_composition
               symrun_interp_expansion inf_assoc inf_left_commute)
 
 text \<open>
-  When there are no constraints on the present left, the interpretation of
+  When there are no remaining constraints on the present, the interpretation of
   a configuration is the same as the configuration at the next instant of its future.
   This corresponds to the introduction rule of the operational semantics.
 \<close>
